examples/ironHT/AbstractService.s.dfy
@@ -1,0 +1,129 @@
+include "AbstractService.s.dfy"
+include "AppInterface.s.dfy"
+include "HT.s.dfy"
+
+module AbstractServiceSHT_s refines AbstractService_s {
+import opened Bytes_s
+import opened AppInterface_i`Spec
+import opened SHT__HT_s
+export Spec
+    provides Native__Io_s, Environment_s, Native__NativeTypes_s
+    provides ServiceState 
+    provides Service_Init, Service_Next, Service_Correspondence
+
+    reveals AppRequest, AppReply
+    provides AppInterface_i, SHT__HT_s
+    provides MarshallServiceGetRequest, MarshallServiceSetRequest, MarshallServiceReply
+export All reveals *
+
+datatype AppRequest = AppGetRequest(g_seqno:int, g_k:Key) | AppSetRequest(s_seqno:int, s_k:Key, ov:OptionalValue)
+datatype AppReply   = AppReply(seqno:int, k:Key, ov:OptionalValue)
+    
+datatype ServiceState' = ServiceState'(
+    serverAddresses:set<EndPoint>,
+    ht:Hashtable,
+    requests:set<AppRequest>,
+    replies:set<AppReply>
+    )
+
+type ServiceState = ServiceState'
+
+predicate Service_Init(s:ServiceState, serverAddresses:set<EndPoint>)
+{
+       s.serverAddresses == serverAddresses
+    && SpecInit(s.ht)
+    && s.requests == {}
+    && s.replies == {}
+}
+
+/*predicate Service_Next_ServerReceivesRequest(s:ServiceState, s':ServiceState, req:AppRequest)
+{
+    s'.requests == s.requests + { req }
+}*/
+
+predicate Service_Next_ServerExecutesRequest(s:ServiceState, s':ServiceState, req:AppRequest, rep:AppReply)
+// ???: seqno
+{
+       s'.serverAddresses == s.serverAddresses
+    && s'.requests == s.requests + { req }
+    && (req.AppGetRequest? ==> Get(s.ht, s'.ht, req.g_k, rep.ov) && s'.replies == s.replies + { rep } && req.g_k == rep.k)
+    && (req.AppSetRequest? ==> Set(s.ht, s'.ht, req.s_k, req.ov) && s'.replies == s.replies + { rep } && req.s_k == rep.k && req.ov == rep.ov)
+}
+
+
+predicate Service_Next(s:ServiceState, s':ServiceState)
+{
+    exists request, reply :: Service_Next_ServerExecutesRequest(s, s', request, reply)
+    //|| exists request :: Service_Next_ServerReceivesRequest(s, s', request)
+}
+
+function MarshallServiceGetRequest(app:AppRequest, reserved:seq<byte>) : seq<byte>
+    requires app.AppGetRequest?
+{
+    if 0 <= app.g_seqno < 0x1_0000_0000_0000_0000 && |reserved| < 0x10_0000 then
+        [ 0, 0, 0, 0, 0, 0, 0, 0] // CSingleMessage_grammar magic number        
+      + Uint64ToBytes(app.g_seqno as uint64)
+      + Uint64ToBytes(|reserved| as uint64)
+      + reserved
+      + [ 0, 0, 0, 0, 0, 0, 0, 0] // CMessage_GetRequest_grammar magic number
+      + MarshallSHTKey(app.g_k)
+    else
+        [ 1 ]
+}
+
+function MarshallServiceSetRequest(app:AppRequest, reserved:seq<byte>) : seq<byte>
+    requires app.AppSetRequest?
+{    
+    if 0 <= app.s_seqno < 0x1_0000_0000_0000_0000 && |reserved| < 0x10_0000 then
+        [ 0, 0, 0, 0, 0, 0, 0, 0] // CSingleMessage_grammar magic number        
+      + Uint64ToBytes(app.s_seqno as uint64)
+      + Uint64ToBytes(|reserved| as uint64)
+      + reserved
+      + [ 0, 0, 0, 0, 0, 0, 0, 1] // CMessage_SetRequest_grammar magic number
+      + MarshallSHTKey(app.s_k)
+      + if app.ov.ValuePresent? then
+            [ 0, 0, 0, 0, 0, 0, 0, 0] // ValuePresent magic number
+            + MarshallSHTValue(app.ov.v)
+        else
+            [ 0, 0, 0, 0, 0, 0, 0, 1] // ValueAbsent magic number
+    else
+        [ 1 ]
+}
+
+function MarshallServiceReply(app:AppReply, reserved:seq<byte>) : seq<byte>
+{
+    if 0 <= app.seqno < 0x1_0000_0000_0000_0000 && |reserved| < 0x10_0000 then
+        [ 0, 0, 0, 0, 0, 0, 0, 0] // CSingleMessage_grammar magic number        
+      + Uint64ToBytes(app.seqno as uint64)
+      + Uint64ToBytes(|reserved| as uint64)
+      + reserved
+      + [ 0, 0, 0, 0, 0, 0, 0, 2] // CMessage_Reply_grammar magic number
+      + MarshallSHTKey(app.k)
+      + if app.ov.ValuePresent? then
+            [ 0, 0, 0, 0, 0, 0, 0, 0] // ValuePresent magic number
+            + MarshallSHTValue(app.ov.v)
+        else
+            [ 0, 0, 0, 0, 0, 0, 0, 1] // ValueAbsent magic number
+    else
+        [ 1 ]
+}
+
+predicate Service_Correspondence(concretePkts:set<LPacket<EndPoint, seq<byte>>>, serviceState:ServiceState) 
+{
+       (forall p, reply, reserved_bytes :: 
+                    p in concretePkts 
+                 && p.src in serviceState.serverAddresses 
+                 && p.msg == MarshallServiceReply(reply, reserved_bytes)
+                 && |reserved_bytes| < 0x10_0000
+                    ==> reply in serviceState.replies)
+    && (forall req :: req in serviceState.requests && req.AppGetRequest? 
+                      ==> exists p, reserved_bytes :: p in concretePkts && p.dst in serviceState.serverAddresses 
+                                                   && p.msg == MarshallServiceGetRequest(req, reserved_bytes)
+                                                   && |reserved_bytes| < 0x10_0000)
+    && (forall req :: req in serviceState.requests && req.AppSetRequest? 
+                      ==> exists p, reserved_bytes :: p in concretePkts && p.dst in serviceState.serverAddresses 
+                                                   && p.msg == MarshallServiceSetRequest(req, reserved_bytes)
+                                                   && |reserved_bytes| < 0x10_0000)
+}
+
+}
