examples/ironLock/test_self.dfy
@@ -1,0 +1,15 @@
+include "service.dfy"
+
+lemma Service_Self_Test() {
+
+    var serverAddresses := {EndPoint([1,2]),EndPoint([1]),EndPoint([3,4]),EndPoint([4])};
+    var s := ServiceState'({EndPoint([1,2]),EndPoint([1]),EndPoint([3,4]),EndPoint([4])}, [EndPoint([1])]);
+    var s' := ServiceState'({EndPoint([1,2]),EndPoint([1]),EndPoint([3,4]),EndPoint([4])}, [EndPoint([1]), EndPoint([1])]);
+
+    // original spec
+    assert Service_Next(s, s');
+
+    // new lock holder
+    assert forall new_lock_holder | new_lock_holder in s.hosts :: new_lock_holder == s.history[|s.history| - 1] || s'.history[|s'.history| - 1] != new_lock_holder;
+    assert !Service_Next_More_Constrained(s, s');
+}
