examples/ironRSL/service.dfy
@@ -1,0 +1,67 @@
+module Native__NativeTypes_s {
+newtype{:nativeType "sbyte"} sbyte = i:int | -0x80 <= i < 0x80
+newtype{:nativeType "byte"} byte = i:int | 0 <= i < 0x100
+newtype{:nativeType "short"} int16 = i:int | -0x8000 <= i < 0x8000
+newtype{:nativeType "ushort"} uint16 = i:int | 0 <= i < 0x10000
+newtype{:nativeType "int"} int32 = i:int | -0x80000000 <= i < 0x80000000
+newtype{:nativeType "uint"} uint32 = i:int | 0 <= i < 0x100000000
+newtype{:nativeType "long"} int64 = i:int | -0x8000000000000000 <= i < 0x8000000000000000
+newtype{:nativeType "ulong"} uint64 = i:int | 0 <= i < 0x10000000000000000
+
+newtype{:nativeType "sbyte"} nat8 = i:int | 0 <= i < 0x80
+newtype{:nativeType "short"} nat16 = i:int | 0 <= i < 0x8000
+newtype{:nativeType "int"} nat32 = i:int | 0 <= i < 0x80000000
+newtype{:nativeType "long"} nat64 = i:int | 0 <= i < 0x8000000000000000
+
+} 
+
+import opened Native__NativeTypes_s
+
+datatype EndPoint = EndPoint(public_key:seq<byte>)
+
+type Bytes = seq<byte>
+type AppState = Bytes
+type AppRequest = Bytes
+type AppReply = Bytes
+
+function AppInitialize() : AppState
+{
+    []
+}
+function AppHandleRequest(m:AppState, request:AppRequest) : (AppState, AppReply)
+{
+    ([],[])
+}
+function method MaxAppRequestSize() : int  { 0x800_0000 }            // 128 MB
+function method MaxAppReplySize() : int    { 0x800_0000 }            // 128 MB
+function method MaxAppStateSize() : int    { 0x1000_0000_0000_0000 } // 2^60 B
+
+datatype AppRequestMessage = AppRequestMessage(client:EndPoint, seqno:int, request:AppRequest)
+datatype AppReplyMessage   = AppReplyMessage(client:EndPoint, seqno:int, reply:AppReply)
+
+datatype ServiceState' = ServiceState'(
+  serverAddresses:set<EndPoint>,
+  app:AppState,
+  requests:set<AppRequestMessage>,
+  replies:set<AppReplyMessage>
+  )
+
+type ServiceState = ServiceState'
+
+predicate Service_Init(s:ServiceState, serverAddresses:set<EndPoint>)
+{
+  && s.serverAddresses == serverAddresses
+  && s.app == AppInitialize()
+  && s.requests == {}
+  && s.replies == {}
+}
+
+predicate ServiceExecutesAppRequest(s:ServiceState, s':ServiceState, req:AppRequestMessage)
+// seqno requirement?
+{
+  && |req.request| <= MaxAppRequestSize()
+  && s'.serverAddresses == s.serverAddresses
+  && s'.requests == s.requests + { req }
+  && s'.app == AppHandleRequest(s.app, req.request).0
+  && s'.replies == s.replies + { AppReplyMessage(req.client, req.seqno, AppHandleRequest(s.app, req.request).1) }
+}
