examples/ironRSL/test_service.dfy
@@ -1,0 +1,18 @@
+include "service.dfy"
+
+import opened Native__NativeTypes_s
+
+lemma TestInit() {
+    var serverAddresses:set<EndPoint> := {EndPoint([0]), EndPoint([0, 0])};
+    var ss := ServiceState'(serverAddresses, [], {}, {});
+    assert Service_Init(ss, serverAddresses);
+
+    var ss2 := ServiceState'(serverAddresses, [1], {}, {});
+    assert !Service_Init(ss2, serverAddresses);
+    
+}
+
+lemma TestExecute() {
+
+}
+
